Semantic/CoreCapybara/Capybara/TypeSystem/Core.lean
@@ -239,6 +239,8 @@ inductive CapyHasType : CaptureSet s -> CapyCtx s -> CapyExp s -> CapyTy .exi s 
     (.typ (.cell (.var (.M .ro) (.bound x)) .ro))
 | fresh :
   CapyHasType C Γ (.var x) (.typ (T.subst (CapySubst.openCVar D))) ->
+  D.IsClosed ->
+  CapyCaptureBound.IsValid Γ (.bound D) ->
   CapyCaptureSet.droppable Γ D ->
   --------------------------------
   CapyHasType (C ∪ D ∪ D.applyDrop) Γ (.var x) (.exi T)
